Fixed while case + formatting

hoare_wp.fst
@@ -503,9 +503,8 @@ Case: c = while be do c' inv i  (TODO)
 ------------------------------
 *)
 
-(* Weakest precondition property : it is false for now, but it should
-   be true without While.  for now, I do not know how to change this
-   definition in order to make it works *)
+(* Weakest precondition property; first semantically (failed attempt),
+                                  then syntactically *)
 
 opaque val skip : p : pred ->  q : pred -> hpcq : hoare p Skip q -> h : heap ->
                   deduce (p h) ->
@@ -675,76 +674,135 @@ type hoare_syn : pred -> com -> pred -> Type =
   | HoareSynWhile : p:pred -> be:bexp -> c:com ->
                     hoare_syn (pand p (bpred be)) c p ->
                     Tot (hoare_syn p (While be c p) (pand p (pnot (bpred be))))
-(* (q'=>q) => (wlp c q' => wlp c q) *)
-assume val impl_wlp : c:com -> q:pred -> q':pred -> deduce(pred_impl q' q) -> Tot(deduce(pred_impl (wlp c q') (wlp c q)))
 
-(* CH: here is a version of wlp_weakest that has some chance of holding *)
+(* (q'=>q) => (wlp c q' => wlp c q) *)
+assume val impl_wlp : c:com -> q:pred -> q':pred ->
+                      deduce (pred_impl q' q) ->
+                      Tot (deduce (pred_impl (wlp c q') (wlp c q)))
+
 (* (p1 => p2) -> (p2 => p3) -> (p1 => p3)*)
-assume val impl_comp : p1 : pred -> p2 : pred -> p3 : pred -> deduce(pred_impl p1 p2) -> deduce (pred_impl p2 p3) -> Tot(deduce (pred_impl p1 p3))
+assume val impl_comp : p1 : pred -> p2 : pred -> p3 : pred ->
+                       deduce (pred_impl p1 p2) ->
+                       deduce (pred_impl p2 p3) ->
+                       Tot (deduce (pred_impl p1 p3))
 
 (*p,be |- wlp body p*)
-val while1' : be : bexp -> body : com -> p : pred -> deduce (pred_impl (pand p (bpred be)) (wlp body p)) -> h : heap -> deduce (p h) -> deduce (bpred be h) -> Tot(deduce (wlp body p h))
+opaque val while1' : be : bexp -> body : com -> p : pred ->
+                     deduce (pred_impl (pand p (bpred be)) (wlp body p)) ->
+                     h : heap -> deduce (p h) -> deduce (bpred be h) ->
+                     Tot (deduce (wlp body p h))
 let while1' be body p vpbewlp h vph vbe =
-let vpbewlph = DForallElim (pimpl (pand p (bpred be)) (wlp body p)) vpbewlp h in
-let vand = DAndIntro (p h) (bpred be h) vph vbe in
-DImplElim (pand p (bpred be) h) (wlp body p h) vpbewlph vand
-val while2' : be : bexp -> body : com -> p : pred -> deduce (pred_impl (pand p (bpred be)) (wlp body p)) -> h : heap -> deduce (p h) -> Tot(deduce (FImpl (bpred be h) (wlp body p h)))
+  let vpbewlph = DForallElim (pimpl (pand p (bpred be)) (wlp body p)) vpbewlp h in
+  let vand = DAndIntro (p h) (bpred be h) vph vbe in
+  DImplElim (pand p (bpred be) h) (wlp body p h) vpbewlph vand
+
+opaque val while2' : be : bexp -> body : com -> p : pred ->
+                     deduce (pred_impl (pand p (bpred be)) (wlp body p)) ->
+                     h : heap -> deduce (p h) ->
+                     Tot (deduce (FImpl (bpred be h) (wlp body p h)))
 let while2' be body p vpbewlp h vph =
-DImplIntro (bpred be h) (wlp body p h) (while1' be body p vpbewlp h vph)
+  DImplIntro (bpred be h) (wlp body p h) (while1' be body p vpbewlp h vph)
 
-val while3' : be : bexp -> body : com -> p : pred -> deduce (pred_impl (pand p (bpred be)) (wlp body p)) -> h : heap -> deduce (p h) -> deduce (pnot (bpred be) h) -> Tot(deduce (FAnd (p h) (pnot (bpred be) h) ))
+opaque val while3' : be : bexp -> body : com -> p : pred ->
+                     deduce (pred_impl (pand p (bpred be)) (wlp body p)) ->
+                     h : heap -> deduce (p h) -> deduce (pnot (bpred be) h) ->
+                     Tot (deduce (FAnd (p h) (pnot (bpred be) h) ))
 let while3' be body p vpbewlp h vph vnbe =
-DAndIntro (p h) (pnot (bpred be) h) vph vnbe
+  DAndIntro (p h) (pnot (bpred be) h) vph vnbe
 
-val while4' : be : bexp -> body : com -> p : pred -> deduce (pred_impl (pand p (bpred be)) (wlp body p)) -> h : heap -> deduce (p h) -> Tot(deduce (FImpl (pnot (bpred be) h) (pand p (pnot (bpred be)) h)))
+opaque val while4' : be : bexp -> body : com -> p : pred ->
+                     deduce (pred_impl (pand p (bpred be)) (wlp body p)) ->
+                     h : heap -> deduce (p h) ->
+                     Tot (deduce (FImpl (pnot (bpred be) h)
+                                        (pand p (pnot (bpred be)) h)))
 let while4' be body p vpbewlp h vph =
-DImplIntro (pnot (bpred be) h) (pand p (pnot (bpred be)) h) (while3' be body p vpbewlp h vph)
+  DImplIntro (pnot (bpred be) h) (pand p (pnot (bpred be)) h)
+             (while3' be body p vpbewlp h vph)
 
 (*
-val while5' : be : bexp -> body : com -> p : pred -> deduce (pred_impl (pand p (bpred be)) (wlp body p)) -> h : heap -> deduce (p h) -> Tot(deduce (FAnd (pimpl (bpred be) (wlp body p) h) (pimpl (pnot (bpred be)) (pand p (pnot (bpred be))) h)))
-
+val while5' : be : bexp -> body : com -> p : pred ->
+              deduce (pred_impl (pand p (bpred be)) (wlp body p)) ->
+              h : heap -> deduce (p h) ->
+              Tot (deduce (FAnd (pimpl (bpred be) (wlp body p) h)
+                                (pimpl (pnot (bpred be))
+                                       (pand p (pnot (bpred be))) h)))
 let while5' be body p vpbewlp h vph vbe iaun =
-DAndIntro (pimpl (bpred be) (wlp body p) h) (pimpl (pnot (bpred be)) (pand p (pnot (bpred be))) h) (while2' be body p vpbewlp h vph) (while4' be body p vpbewlp h vph)
-
+  DAndIntro (pimpl (bpred be) (wlp body p) h)
+            (pimpl (pnot (bpred be)) (pand p (pnot (bpred be))) h)
+            (while2' be body p vpbewlp h vph) (while4' be body p vpbewlp h vph)
 *)
-val while6' : be : bexp -> body : com -> p : pred -> deduce (pred_impl (pand p (bpred be)) (wlp body p)) -> h : heap -> Tot(deduce (FImpl (p h) (FAnd (pimpl (bpred be) (wlp body p) h) (pimpl (pnot (bpred be)) (pand p (pnot (bpred be))) h))))
-let while6' be body p vpbewlp h =
-DImplIntro (p h) (FAnd (pimpl (bpred be) (wlp body p) h) (pimpl (pnot (bpred be)) (pand p (pnot (bpred be))) h)) (fun vph -> 
-DAndIntro (pimpl (bpred be) (wlp body p) h) (pimpl (pnot (bpred be)) (pand p (pnot (bpred be))) h) (while2' be body p vpbewlp h vph) (while4' be body p vpbewlp h vph))
-val while7' : be : bexp -> body : com -> p : pred -> deduce (pred_impl (pand p (bpred be)) (wlp body p)) -> h : heap -> deduce (p h) -> Tot(deduce (FAnd (p h) (pred_impl (p) (pand (pimpl (bpred be) (wlp body p) ) (pimpl (pnot (bpred be)) (pand p (pnot (bpred be))) )))))
-let while7' be body p vpbewlp h vph =
-DAndIntro (p h) (pred_impl (p) (pand (pimpl (bpred be) (wlp body p) ) (pimpl (pnot (bpred be)) (pand p (pnot (bpred be))) ))) vph (DForallIntro (pimpl p (pand (pimpl (bpred be) (wlp body p) ) (pimpl (pnot (bpred be)) (pand p (pnot (bpred be))) ))) (while6' be body p vpbewlp))
-val while8' : be : bexp -> body : com -> p : pred -> deduce (pred_impl (pand p (bpred be)) (wlp body p)) -> h : heap ->  
-Tot(deduce (FImpl (p h) (FAnd (p h) (pred_impl (p) (pand (pimpl (bpred be) (wlp body p) ) (pimpl (pnot (bpred be)) (pand p (pnot (bpred be))) ))))))
-let while8' be body p vpbewlp h =
-DImplIntro (p h) (pand p (fun _ -> pred_impl (p) (pand (pimpl (bpred be) (wlp body p) ) (pimpl (pnot (bpred be)) (pand p (pnot (bpred be))) ))) h) (while7' be body p vpbewlp h)
 
+opaque val while6' : be : bexp -> body : com -> p : pred ->
+                     deduce (pred_impl (pand p (bpred be)) (wlp body p)) ->
+                     h : heap ->
+  Tot (deduce (FImpl (p h) (FAnd (pimpl (bpred be) (wlp body p) h)
+                                 (pimpl (pnot (bpred be))
+                                        (pand p (pnot (bpred be))) h))))
+let while6' be body p vpbewlp h =
+  DImplIntro (p h) (FAnd (pimpl (bpred be) (wlp body p) h)
+                         (pimpl (pnot (bpred be)) (pand p (pnot (bpred be))) h))
+             (fun vph -> DAndIntro (pimpl (bpred be) (wlp body p) h)
+                                   (pimpl (pnot (bpred be))
+                                          (pand p (pnot (bpred be))) h)
+                                   (while2' be body p vpbewlp h vph)
+                                   (while4' be body p vpbewlp h vph))
+
+opaque val while7' : be : bexp -> body : com -> p : pred ->
+                     deduce (pred_impl (pand p (bpred be)) (wlp body p)) ->
+                     h : heap -> deduce (p h) ->
+                     Tot (deduce (FAnd (p h) (pred_impl (p)
+                                          (pand (pimpl (bpred be) (wlp body p))
+                                          (pimpl (pnot (bpred be))
+                                                 (pand p (pnot (bpred be))))))))
+let while7' be body p vpbewlp h vph =
+  DAndIntro (p h) (pred_impl (p) (pand (pimpl (bpred be) (wlp body p) )
+                                       (pimpl (pnot (bpred be))
+                                              (pand p (pnot (bpred be))) )))
+            vph (DForallIntro (pimpl p (pand (pimpl (bpred be) (wlp body p) )
+                                             (pimpl (pnot (bpred be))
+                                                    (pand p (pnot (bpred be))) )))
+                              (while6' be body p vpbewlp))
+
+opaque val while8' : be : bexp -> body : com -> p : pred ->
+                     deduce (pred_impl (pand p (bpred be)) (wlp body p)) ->
+                     h : heap ->
+                     Tot (deduce (FImpl (p h) (FAnd (p h) (pred_impl (p)
+                                  (pand (pimpl (bpred be) (wlp body p) )
+                                        (pimpl (pnot (bpred be))
+                                               (pand p (pnot (bpred be))) ))))))
+let while8' be body p vpbewlp h =
+  let aux _ = pred_impl p (pand (pimpl (bpred be) (wlp body p) )
+                                (pimpl (pnot (bpred be))
+                                       (pand p (pnot (bpred be))) )) in
+  DImplIntro (p h) (pand p aux h) (while7' be body p vpbewlp h)
 
 opaque val wlp_weakest' : c:com -> p:pred -> q:pred ->
                          hpcq:hoare_syn p c q ->
                          Tot (deduce (pred_impl p (wlp c q))) (decreases hpcq)
 let rec wlp_weakest' c p q hpcq =
   match hpcq with
-(*p = pred_sub x e q*)
-  | HoareSynAssign q' x e -> DForallIntro (pimpl p p) (fun h -> DImplIntro (p h) (p h) (plouf p h)) 
+  | HoareSynAssign q' x e ->
+     DForallIntro (pimpl p p) (fun h -> DImplIntro (p h) (p h) (plouf p h))
   | HoareSynConsequence p' p'' q' q'' c' hc vpp' vq'q ->
-   let impl3 = impl_wlp c' q' q'' vq'q in
-   let impl2 = wlp_weakest' c p'' q'' hc in
-   let vpwlp' = impl_comp p' p'' (wlp c q'') vpp' impl2 in
-   impl_comp p' (wlp c q'') (wlp c q') vpwlp' impl3  
-  | HoareSynSkip p' -> DForallIntro (pimpl p' p') (fun h -> DImplIntro (p' h) (p' h) (plouf p' h))
-  | HoareSynSeq p' c1 q' c2  r' hc1 hc2 -> 
-   let implqwlpc2 = wlp_weakest' c2 q' r' hc2 in
-   let implwlpc1 = impl_wlp c1 (wlp c2 r') q' implqwlpc2 in
-   let implpwlp = wlp_weakest' c1 p' q' hc1 in
-   impl_comp p' (wlp c1 q') (wlp c1 (wlp c2 r')) implpwlp implwlpc1
-  | HoareSynIf p' q' be ct ce hct hce -> 
-    let vimpltrue = wlp_weakest' ct (pand p' (bpred be)) q' hct in
-    let vimplfalse = wlp_weakest' ce (pand p' (pnot (bpred be))) q' hce in
-    if1 be ct ce p' q' vimpltrue vimplfalse 
-  | HoareSynWhile p be body hbody -> let vimplbody = wlp_weakest' body (pand p (bpred be)) p hbody in
-    let prop = DForallIntro (pimpl p (pand (pimpl (bpred be) (wlp body p)) (pimpl (pnot (bpred be)) (pand p (pnot (bpred be)))))) (while6' be body p vimplbody) in
-magic()
-(*
-    DForallIntro (pimpl p  (pand p (fun _ -> pred_impl (p) (pand (pimpl (bpred be) (wlp body p) ) (pimpl (pnot (bpred be)) (pand p (pnot (bpred be))) )))) ) (while8' be body p vimplbody)
-*)
+     let impl3 = impl_wlp c' q' q'' vq'q in
+     let impl2 = wlp_weakest' c p'' q'' hc in
+     let vpwlp' = impl_comp p' p'' (wlp c q'') vpp' impl2 in
+     impl_comp p' (wlp c q'') (wlp c q') vpwlp' impl3
+  | HoareSynSkip p' ->
+     DForallIntro (pimpl p' p') (fun h -> DImplIntro (p' h) (p' h) (plouf p' h))
+  | HoareSynSeq p' c1 q' c2  r' hc1 hc2 ->
+     let implqwlpc2 = wlp_weakest' c2 q' r' hc2 in
+     let implwlpc1 = impl_wlp c1 (wlp c2 r') q' implqwlpc2 in
+     let implpwlp = wlp_weakest' c1 p' q' hc1 in
+     impl_comp p' (wlp c1 q') (wlp c1 (wlp c2 r')) implpwlp implwlpc1
+  | HoareSynIf p' q' be ct ce hct hce ->
+     let vimpltrue = wlp_weakest' ct (pand p' (bpred be)) q' hct in
+     let vimplfalse = wlp_weakest' ce (pand p' (pnot (bpred be))) q' hce in
+     if1 be ct ce p' q' vimpltrue vimplfalse
+  | HoareSynWhile p be body hbody ->
+     let vimplbody = wlp_weakest' body (pand p (bpred be)) p hbody in
+     let prop = DForallIntro (pimpl p (pand (pimpl (bpred be) (wlp body p))
+                                            (pimpl (pnot (bpred be))
+                                                   (pand p (pnot (bpred be))))))
+                             (while6' be body p vimplbody) in
+     DForallIntro (pimpl p (wlp c q)) (while8' be body p vimplbody)
